src/program_proof/marshal_block.v
@@ -1,0 +1,50 @@
+From Goose.github_com.tchajed Require Import marshal.
+
+From Perennial.program_proof Require Import proof_prelude.
+From Perennial.program_proof Require Import disk_lib.
+From Perennial.program_proof Require Import marshal_proof_new.
+From Perennial.goose_lang.lib Require Import slice.typed_slice.
+
+Definition block_encodes (b:Block) r :=
+  has_encoding (vec_to_list b) r.
+
+Typeclasses Opaque block_encodes.
+
+Section goose_lang.
+Context `{!heapG Σ}.
+
+Notation is_benc enc_v r remaining :=
+  (is_enc enc_v 4096 r remaining).
+
+Theorem wp_Enc__Finish_block stk E enc_v r remaining :
+  {{{ is_benc enc_v r remaining }}}
+    Enc__Finish enc_v @ stk; E
+  {{{ s b, RET slice_val s; is_block s 1 b ∗ ⌜block_encodes b r⌝ }}}.
+Proof.
+  iIntros (Φ) "Hpre HΦ".
+  wp_apply (wp_Enc__Finish with "Hpre").
+  iIntros (??) "(%Henc&%Hdatalen&Hs)".
+  iApply ("HΦ" $! _ (list_to_block data)).
+  iSplitL.
+  - iApply is_slice_to_small in "Hs".
+    rewrite /is_slice_small /is_block.
+    rewrite -> list_to_block_to_vals by word.
+    iFrame.
+  - rewrite /block_encodes.
+    iPureIntro.
+    rewrite list_to_block_to_list //.
+Qed.
+
+Theorem wp_new_dec_block stk E s q b r :
+  block_encodes b r →
+  {{{ is_block s q b }}}
+    NewDec (slice_val s) @ stk; E
+  {{{ dec_v, RET dec_v; is_dec dec_v r }}}.
+Proof.
+  iIntros (Henc Φ) "Hpre HΦ".
+  wp_apply (wp_new_dec with "Hpre"); eauto.
+Qed.
+
+End goose_lang.
+
+Opaque block_encodes.
